Add support for SMT triggers
This is implemented by allowing arbitrary attributes to be
propagated throughout the pipeline. For the SMT backend, these are
translated into SMT attributes. Currently, the only attribute supported
is the `:pattern` attribute used to indicate triggers. Adding other
attributes will be easy now that this plumbing is in place, however.

Attributes currently aren't supported for TPTP, but it should be
possible to allow them eventually if there's a use for them.

Note that the initial construction of attributes is very general, and
allows attributes of any base type supported by the translator. The set
supported by SMT is more restricted, but other prover input languages
may use entirely different attributes.

There's no attempt to ensure that attributes go in places that are
allowed. So, for instance, adding a trigger outside of a quantified
expression will lead to an error from the solver. Similarly, adding a
trigger to a goal, rather than an axiom, will typically also lead to an
error.

Auto/Embedding/LamBase.lean
@@ -1418,6 +1418,90 @@ def BitVecConst.LamWF.ofCheck (H : b.lamCheck = s) : LamWF b s := by
   case bvcmp n prop? op => cases prop? <;> constructor
   case bvshOp n smt? op => cases smt? <;> constructor
 
+inductive OtherConst
+  | attribute : String -> LamSort -> OtherConst
+deriving Inhabited, Hashable, Lean.ToExpr
+
+def OtherConst.reprAux : OtherConst → String
+| .attribute n s => s!"attribute {n} {s}"
+
+def OtherConst.reprPrec (p : OtherConst) (n : Nat) :=
+  match n with
+  | 0 => f!"Auto.Embedding.Lam.OtherConst.{p.reprAux}"
+  | _ + 1 => f!"(.{p.reprAux})"
+
+inductive OtherConst.LamWF : OtherConst → LamSort → Type
+  | ofAttribute n s    : LamWF (.attribute n s) (.func s (.func (.base .prop) (.base .prop)))
+
+def OtherConst.LamWF.ofOtherConst : (oc : OtherConst) → (s : LamSort) × OtherConst.LamWF oc s
+| .attribute n s  => ⟨.func s (.func (.base .prop) (.base .prop)), .ofAttribute n s⟩
+
+def OtherConst.LamWF.interp (tyVal : Nat → Type u) : (lwf : LamWF p s) → s.interp tyVal
+| .ofAttribute _ _ =>  fun _ => fun term => term
+
+def OtherConst.toString : OtherConst → String
+| .attribute n s => s!"attr[{n} : {s}]"
+
+instance : ToString OtherConst where
+  toString := OtherConst.toString
+
+def OtherConst.beq : OtherConst → OtherConst → Bool
+| .attribute n1 s1, .attribute n2 s2 =>
+  n1 == n2 && s1.beq s2
+
+instance : BEq OtherConst where
+  beq := OtherConst.beq
+
+theorem OtherConst.beq_def {x y : OtherConst} : (x == y) = x.beq y := rfl
+
+def OtherConst.beq_refl {o : OtherConst} : (o.beq o) = true := by
+  cases o <;> unfold OtherConst.beq <;> simp [LamSort.beq_refl]
+
+def OtherConst.eq_of_beq_eq_true {o₁ o₂ : OtherConst} (H : o₁.beq o₂) : o₁ = o₂ :=
+  match o₁, o₂ with
+  | .attribute n1 s1, .attribute n2 s2 => by
+    simp [OtherConst.beq] at H
+    match H with
+    | And.intro neq sbeq =>
+      have seq := LamSort.eq_of_beq_eq_true sbeq
+      rw [neq, seq]
+
+instance : LawfulBEq OtherConst where
+  eq_of_beq := OtherConst.eq_of_beq_eq_true
+  rfl := OtherConst.beq_refl
+
+def OtherConst.lamCheck : OtherConst → LamSort
+| .attribute _ as1 => .func as1 (.func (.base .prop) (.base .prop))
+
+-- Note: add other attributes as needed
+def trigger {a : Type} (_ : a) (term : Prop) := term
+
+def OtherConst.interp (tyVal : Nat → Type u) : (o : OtherConst) → o.lamCheck.interp tyVal
+| .attribute _ _ => fun _ => fun term => term
+
+def OtherConst.interp_equiv (tyVal : Nat → Type u) (ocwf : LamWF p s) :
+  HEq (LamWF.interp tyVal ocwf) (interp tyVal p) := by
+  cases ocwf <;> rfl
+
+def OtherConst.LamWF.unique {o : OtherConst} {s₁ s₂ : LamSort}
+  (ocwf₁ : LamWF o s₁) (ocwf₂ : LamWF o s₂) : s₁ = s₂ ∧ HEq ocwf₁ ocwf₂ := by
+  cases ocwf₁ <;> cases ocwf₂ <;> trivial
+
+theorem OtherConst.LamWF.interp_lvalIrrelevance
+  (tyVal₁ tyVal₂ : Nat → Type u) (ocwf₁ : LamWF b₁ s₁) (ocwf₂ : LamWF b₂ s₂)
+  (HBeq : b₁ = b₂) (hTyVal : tyVal₁ = tyVal₂) :
+  HEq (ocwf₁.interp tyVal₁) (ocwf₂.interp tyVal₂) := by
+  cases HBeq; cases hTyVal; rcases OtherConst.LamWF.unique ocwf₁ ocwf₂ with ⟨⟨⟩, ⟨⟩⟩; rfl
+
+def OtherConst.lamWF_complete (wf : LamWF sc s) : LamWF.ofOtherConst sc = ⟨s, wf⟩ := by
+  cases wf <;> rfl
+
+def OtherConst.lamCheck_of_LamWF (H : LamWF sc s) : sc.lamCheck = s := by
+  cases H <;> rfl
+
+def OtherConst.LamWF.ofCheck (H : sc.lamCheck = s) : LamWF sc s := by
+  cases H; cases sc <;> constructor
+
 /--
   Interpreted constants
   Note that `eq`, `forallE`, `existE` have `ilVal/lamILTy`
@@ -1442,6 +1526,7 @@ inductive LamBaseTerm
   | icst     : IntConst    → LamBaseTerm
   | scst     : StringConst → LamBaseTerm
   | bvcst    : BitVecConst → LamBaseTerm
+  | ocst     : OtherConst  → LamBaseTerm
   -- Versions of `eq, ∀, ∃, ite'` when we're importing external facts
   -- Note that the [import versions] of `eq, ∀, ∃, ite'` should only be used when
   --   we're importing external facts. When facts are imported, we call
@@ -1604,6 +1689,7 @@ def LamBaseTerm.reprPrec (l : LamBaseTerm) (n : Nat) :=
     | .icst ic    => f!"icst {IntConst.reprPrec ic 1}"
     | .scst sc    => f!"scst {StringConst.reprPrec sc 1}"
     | .bvcst bvc  => f!"bvcst {BitVecConst.reprPrec bvc 1}"
+    | .ocst oc    => f!"ocst {OtherConst.reprPrec oc 1}"
     | .eqI n      => f!"eqI {n}"
     | .forallEI n => f!"forallEI {n}"
     | .existEI n  => f!"existEI {n}"
@@ -1627,6 +1713,7 @@ def LamBaseTerm.toString : LamBaseTerm → String
 | .icst ic    => s!"{ic}"
 | .scst sc    => s!"{sc}"
 | .bvcst bvc  => s!"{bvc}"
+| .ocst oc    => s!"{oc}"
 | .eqI _      => "="
 | .forallEI _ => "∀"
 | .existEI _  => "∃"
@@ -1646,6 +1733,7 @@ def LamBaseTerm.beq : LamBaseTerm → LamBaseTerm → Bool
 | .icst ic₁,    .icst ic₂    => IntConst.beq ic₁ ic₂
 | .scst sc₁,    .scst sc₂    => StringConst.beq sc₁ sc₂
 | .bvcst l₁,    .bvcst l₂    => BitVecConst.beq l₁ l₂
+| .ocst o₁,     .ocst o₂     => OtherConst.beq o₁ o₂
 | .eqI n₁,      .eqI n₂      => n₁.beq n₂
 | .forallEI n₁, .forallEI n₂ => n₁.beq n₂
 | .existEI n₁,  .existEI n₂  => n₁.beq n₂
@@ -1667,6 +1755,7 @@ def LamBaseTerm.beq_refl {b : LamBaseTerm} : (b.beq b) = true := by
   case icst i => apply LawfulBEq.rfl (α := IntConst)
   case scst s => apply LawfulBEq.rfl (α := StringConst)
   case bvcst s => apply LawfulBEq.rfl (α := BitVecConst)
+  case ocst o => apply LawfulBEq.rfl (α := OtherConst)
 
 def LamBaseTerm.eq_of_beq_eq_true {b₁ b₂ : LamBaseTerm} (H : b₁.beq b₂) : b₁ = b₂ := by
   cases b₁ <;> cases b₂ <;> (first | contradiction | rfl | apply congrArg) <;>
@@ -1677,6 +1766,7 @@ def LamBaseTerm.eq_of_beq_eq_true {b₁ b₂ : LamBaseTerm} (H : b₁.beq b₂) 
   case icst.icst.h n₁ n₂ => apply LawfulBEq.eq_of_beq (α := IntConst) H
   case scst.scst.h s₁ s₂ => apply LawfulBEq.eq_of_beq (α := StringConst) H
   case bvcst.bvcst.h v₁ v₂ => apply LawfulBEq.eq_of_beq (α := BitVecConst) H
+  case ocst.ocst.h o₁ o₂ => apply LawfulBEq.eq_of_beq (α := OtherConst) H
 
 instance : LawfulBEq LamBaseTerm where
   eq_of_beq := LamBaseTerm.eq_of_beq_eq_true
@@ -1690,6 +1780,7 @@ def LamBaseTerm.containsSort (b : LamBaseTerm) (s : LamSort) : Bool :=
   | .icst _     => false
   | .scst _     => false
   | .bvcst _    => false
+  | .ocst _     => false
   | .eqI _      => false
   | .forallEI _ => false
   | .existEI _  => false
@@ -1714,6 +1805,7 @@ def LamBaseTerm.lamCheck (ltv : LamTyVal) : LamBaseTerm → LamSort
 | .icst ic    => ic.lamCheck
 | .scst sc    => sc.lamCheck
 | .bvcst bvc  => bvc.lamCheck
+| .ocst oc    => oc.lamCheck
 | .eqI n      =>
   let s := ltv.lamILTy n
   .func s (.func s (.base .prop))
@@ -1738,6 +1830,7 @@ inductive LamBaseTerm.LamWF (ltv : LamTyVal) : LamBaseTerm → LamSort → Type
   | ofIcst       : (icwf : IntConst.LamWF ic s) → LamWF ltv (.icst ic) s
   | ofScst       : (scwf : StringConst.LamWF sc s) → LamWF ltv (.scst sc) s
   | ofBvcst      : (bvcwf : BitVecConst.LamWF bvc s) → LamWF ltv (.bvcst bvc) s
+  | ofOcst       : (ocwf : OtherConst.LamWF oc s) → LamWF ltv (.ocst oc) s
   | ofEqI n      : LamWF ltv (.eqI n) (.func (ltv.lamILTy n) (.func (ltv.lamILTy n) (.base .prop)))
   | ofForallEI n : LamWF ltv (.forallEI n) (.func (.func (ltv.lamILTy n) (.base .prop)) (.base .prop))
   | ofExistEI n  : LamWF ltv (.existEI n) (.func (.func (ltv.lamILTy n) (.base .prop)) (.base .prop))
@@ -1762,6 +1855,8 @@ def LamBaseTerm.LamWF.unique {ltv : LamTyVal} {b : LamBaseTerm} {s₁ s₂ : Lam
     rcases StringConst.LamWF.unique wf₁ wf₂ with ⟨⟨⟩, ⟨⟩⟩; trivial
   case ofBvcst.ofBvcst bvc wf₁ wf₂ =>
     rcases BitVecConst.LamWF.unique wf₁ wf₂ with ⟨⟨⟩, ⟨⟩⟩; trivial
+  case ofOcst.ofOcst oc wf₁ wf₂ =>
+    rcases OtherConst.LamWF.unique wf₁ wf₂ with ⟨⟨⟩, ⟨⟩⟩; trivial
 
 def LamBaseTerm.LamWF.eVarIrrelevance
   (hLamVarTy : ltv₁.lamVarTy = ltv₂.lamVarTy)
@@ -1876,6 +1971,7 @@ def LamBaseTerm.LamWF.ofLamBaseTerm (ltv : LamTyVal) : (b : LamBaseTerm) → (s 
 | .icst ic    => have ⟨s, wf⟩ := IntConst.LamWF.ofIntConst ic; ⟨s, .ofIcst wf⟩
 | .scst sc    => have ⟨s, wf⟩ := StringConst.LamWF.ofStringConst sc; ⟨s, .ofScst wf⟩
 | .bvcst bvc  => have ⟨s, wf⟩ := BitVecConst.LamWF.ofBitVecConst bvc; ⟨s, .ofBvcst wf⟩
+| .ocst oc    => have ⟨s, wf⟩ := OtherConst.LamWF.ofOtherConst oc; ⟨s, .ofOcst wf⟩
 | .eqI n      => ⟨.func _ (.func _ (.base .prop)), .ofEqI n⟩
 | .forallEI n => ⟨.func (.func _ (.base .prop)) (.base .prop), .ofForallEI n⟩
 | .existEI n  => ⟨.func (.func _ (.base .prop)) (.base .prop), .ofExistEI n⟩
@@ -1893,6 +1989,7 @@ def LamBaseTerm.lamWF_complete (wf : LamWF ltv b s) : LamWF.ofLamBaseTerm ltv b 
   case ofIcst ic wf => dsimp [LamWF.ofLamBaseTerm]; rw [IntConst.lamWF_complete]
   case ofScst bc wf => dsimp [LamWF.ofLamBaseTerm]; rw [StringConst.lamWF_complete wf]
   case ofBvcst bc wf => dsimp [LamWF.ofLamBaseTerm]; rw [BitVecConst.lamWF_complete wf]
+  case ofOcst oc wf => dsimp [LamWF.ofLamBaseTerm]; rw [OtherConst.lamWF_complete wf]
 
 def LamBaseTerm.lamCheck_of_LamWF (H : LamWF ltv b s) : b.lamCheck ltv = s := by
   cases H <;> try rfl
@@ -1902,6 +1999,7 @@ def LamBaseTerm.lamCheck_of_LamWF (H : LamWF ltv b s) : b.lamCheck ltv = s := by
   case ofIcst bc wf => apply IntConst.lamCheck_of_LamWF wf
   case ofScst sc wf => apply StringConst.lamCheck_of_LamWF wf
   case ofBvcst sc wf => apply BitVecConst.lamCheck_of_LamWF wf
+  case ofOcst oc wf => apply OtherConst.lamCheck_of_LamWF wf
 
 def LamBaseTerm.LamWF.ofCheck (H : b.lamCheck ltv = s) : LamWF ltv b s := by
   cases H; cases b <;> constructor
@@ -1911,6 +2009,7 @@ def LamBaseTerm.LamWF.ofCheck (H : b.lamCheck ltv = s) : LamWF ltv b s := by
   case refl.icst.icwf => apply IntConst.LamWF.ofCheck; rfl
   case refl.scst.scwf => apply StringConst.LamWF.ofCheck; rfl
   case refl.bvcst.bvcwf => apply BitVecConst.LamWF.ofCheck; rfl
+  case refl.ocst.ocwf => apply OtherConst.LamWF.ofCheck; rfl
 
 structure ILLift (β : Type u) where
   eqL     : EqLift.{u + 1, u} β
@@ -2192,6 +2291,7 @@ noncomputable def LamBaseTerm.interp (lval : LamValuation.{u}) : (b : LamBaseTer
 | .icst ic    => ic.interp lval.tyVal
 | .scst sc    => sc.interp lval.tyVal
 | .bvcst bvc  => bvc.interp lval.tyVal
+| .ocst oc    => oc.interp lval.tyVal
 | .eqI n      => (lval.ilVal n).eqL.eqF
 | .forallEI n => (lval.ilVal n).forallL.forallF
 | .existEI n  => (lval.ilVal n).existL.existF
@@ -2208,6 +2308,7 @@ noncomputable def LamBaseTerm.LamWF.interp (lval : LamValuation.{u}) : (lwf : La
 | .ofIcst wf    => wf.interp lval.tyVal
 | .ofScst wf    => wf.interp lval.tyVal
 | .ofBvcst wf   => wf.interp lval.tyVal
+| .ofOcst wf    => wf.interp lval.tyVal
 | .ofEqI n      => (lval.ilVal n).eqL.eqF
 | .ofForallEI n => (lval.ilVal n).forallL.forallF
 | .ofExistEI n  => (lval.ilVal n).existL.existF
@@ -2254,6 +2355,7 @@ theorem LamBaseTerm.LamWF.interp_lvalIrrelevance
           case ofIcst => apply IntConst.LamWF.interp_lvalIrrelevance <;> rfl
           case ofScst => apply StringConst.LamWF.interp_lvalIrrelevance <;> rfl
           case ofBvcst => apply BitVecConst.LamWF.interp_lvalIrrelevance <;> rfl
+          case ofOcst => apply OtherConst.LamWF.interp_lvalIrrelevance <;> rfl
 
 def LamBaseTerm.interp_equiv (lval : LamValuation.{u})
   (lwf : LamWF lval.toLamTyVal b s) :
@@ -2265,6 +2367,7 @@ def LamBaseTerm.interp_equiv (lval : LamValuation.{u})
   case ofIcst => apply IntConst.interp_equiv
   case ofScst => apply StringConst.interp_equiv
   case ofBvcst => apply BitVecConst.interp_equiv
+  case ofOcst => apply OtherConst.interp_equiv
 
 def LamValuation.insertEVarAt (lval : LamValuation.{u})
   (ty : LamSort) (val : ty.interp lval.tyVal) (pos : Nat) :=
