Auto/Translation/LamReif.lean
@@ -1271,6 +1271,11 @@ def reifMapBVConst3 : HashMap Name (Nat → Nat → Nat → LamTerm) :=
     (``BitVec.extractLsb, fun n h l => .base (.bvextract n h l))
   ]
 
+def reifMapAttributes : HashMap Name String :=
+  HashMap.ofList [
+    (``trigger, "pattern")
+  ]
+
 def processSimpleLit (l : Literal) : LamTerm :=
   match l with
   | .natVal n => .base (.natVal n)
@@ -1307,6 +1312,10 @@ def processSimpleApp (fn arg : Expr) : ReifM (Option LamTerm) := do
       -- `arg` is the original (un-lifted) type
     if let .some tcon := reifMapIL.find? name then
       return .some (.base (tcon (← reifType arg)))
+    if let .some attrName := reifMapAttributes.find? name then
+      if lvls.length != 0 then
+        throwError "processSimpleApp :: attribute should have nil level list"
+      return .some (.base (.ocst (.attribute attrName (← reifType arg))))
     return .none
   | [arg₁, arg₂] =>
     if let .some tcon := reifMapBVConst2.find? name then
